Changed to untyped expressions

kami_rewrites_reflection.v
@@ -6,6 +6,12 @@ Require Import List.
  *
  * Code to perform all the rewrites in kami_rewrites_db by reflection
  *)
+
+Inductive KRElem: Type :=
+| KRRegInitT : KRElem
+| KRRule : KRElem
+| KRMeth : KRElem.
+
 Inductive KRTyp : Type :=
   | KRTypModuleElt: KRTyp
   | KRTypRegInitT: KRTyp
@@ -22,93 +28,203 @@ Fixpoint KRrealizeType (t: KRTyp) :=
   | KRList t => list (KRrealizeType t)
   end.
 
-Inductive KRExp: KRTyp -> Type :=
-  | KRNil t : @KRExp (KRList t)
-  | KRVar t : (KRrealizeType t) -> @KRExp t
-  | KRCons t : @KRExp t -> @KRExp (KRList t) -> @KRExp (KRList t)
-  | KRApp t : @KRExp (KRList t) -> @KRExp (KRList t) -> @KRExp (KRList t)
-  | KRMERegister : @KRExp KRTypRegInitT -> @KRExp KRTypModuleElt
-  | KRRegisters : @KRExp (KRList KRTypRegInitT) -> @KRExp (KRList KRTypModuleElt)
-  | KRMERule : @KRExp KRTypAttributeActionVoid -> @KRExp KRTypModuleElt
-  | KRMEMeth : @KRExp KRTypDefMethT -> @KRExp KRTypModuleElt
-  | KRMakeModule_rules : @KRExp (KRList KRTypModuleElt) -> @KRExp (KRList KRTypAttributeActionVoid)
-  | KRMakeModule_regs : @KRExp (KRList KRTypModuleElt) -> @KRExp (KRList KRTypRegInitT)
-  | KRMakeModule_meths : @KRExp (KRList KRTypModuleElt) -> @KRExp (KRList KRTypDefMethT).
+Inductive KRExp: Type :=
+  | KRNil (t:KRTyp) : @KRExp
+  | KRVar (t:KRTyp) : KRrealizeType t -> @KRExp
+  | KRCons (t:KRTyp) : @KRExp -> @KRExp-> @KRExp
+  | KRApp (t:KRTyp) : @KRExp -> @KRExp -> @KRExp
+  | KRMERegister : @KRExp -> @KRExp
+  | KRRegisters : @KRExp -> @KRExp
+  | KRMERule : @KRExp -> @KRExp
+  | KRMEMeth : @KRExp -> @KRExp
+  | KRMakeModule_rules : @KRExp -> @KRExp
+  | KRMakeModule_regs : @KRExp -> @KRExp
+  | KRMakeModule_meths : @KRExp -> @KRExp.
 
-Fixpoint KRRealizeExp {t} (e: KRExp t) :=
-  match e in KRExp t return (KRrealizeType t) with
-  | KRNil t => @nil (@KRrealizeType t)
-  | KRVar t e => e
-  | KRCons t a b => @cons (@KRrealizeType t) (@KRRealizeExp t a) (@KRRealizeExp (KRList t) b)
-  | KRApp t a b => @app (@KRrealizeType t) (@KRRealizeExp (KRList t) a) (@KRRealizeExp (KRList t) b)
-  | KRMERegister e => MERegister (@KRRealizeExp KRTypRegInitT e)
-  | KRRegisters l => Registers (@KRRealizeExp (KRList KRTypRegInitT) l)
-  | KRMERule r => MERule (@KRRealizeExp KRTypAttributeActionVoid r)
-  | KRMEMeth m => MEMeth (@KRRealizeExp KRTypDefMethT m)
-  | KRMakeModule_rules r => makeModule_rules (@KRRealizeExp (KRList KRTypModuleElt) r)
-  | KRMakeModule_regs r => makeModule_regs (@KRRealizeExp (KRList KRTypModuleElt) r)
-  | KRMakeModule_meths m =>makeModule_meths (@KRRealizeExp (KRList KRTypModuleElt) m)
+Fixpoint KRExpType (e: KRExp) :=
+  match e in KRExp return KRTyp with
+  | KRNil t => KRList t
+  | KRVar t e => t
+  | KRCons t a b => (KRList t)
+  | KRApp t a b => (KRList t)
+  | KRMERegister e => KRTypModuleElt
+  | KRRegisters l => (KRList KRTypModuleElt)
+  | KRMERule r => KRTypModuleElt
+  | KRMEMeth m => KRTypModuleElt
+  | KRMakeModule_rules r => KRList KRTypAttributeActionVoid
+  | KRMakeModule_regs r => KRList KRTypDefMethT
+  | KRMakeModule_meths m => KRList KRTypModuleElt
+  end.
+
+Fixpoint KRRealizeExp {typ} (e: KRExp) : option (KRrealizeType typ).
+refine
+  match e in KRExp return option (@KRrealizeType typ) with
+  | KRNil t => match typ with
+               | KRList x => Some (@nil (KRrealizeType x))
+               | _ => None
+               end
+  | KRVar t e => _
+  | KRCons t a b => match typ,@KRRealizeExp t a,@KRRealizeExp (KRList t) b with
+                    | (KRList t),Some f,Some r => _
+                    | _,_,_ => None
+                    end
+  | KRApp t a b => match typ,@KRRealizeExp (KRList t) a,@KRRealizeExp (KRList t) b with
+                    | (KRList t),Some f,Some r => _
+                    | _,_,_ => None
+                    end
+  | KRMERegister e => match typ,@KRRealizeExp KRTypRegInitT e with
+                     | KRTypModuleElt,Some p => Some (MERegister p)
+                     | _,_ => None
+                     end
+  | KRMERule e => match typ,@KRRealizeExp KRTypAttributeActionVoid e with
+                  | KRTypModuleElt,Some p => Some (MERule p)
+                  | _,_ => None
+                  end
+  | KRMEMeth e => match typ,@KRRealizeExp KRTypDefMethT e with
+                  | KRTypModuleElt,Some p => Some (MEMeth p)
+                  | _,_ => None
+                  end
+  | KRMakeModule_rules e => match typ,@KRRealizeExp (KRList KRTypModuleElt) e with
+                            | (KRList KRTypAttributeActionVoid),Some p => Some (makeModule_rules p)
+                            | _,_ => None
+                            end
+  | KRMakeModule_meths e => match typ,@KRRealizeExp (KRList KRTypModuleElt) e with
+                            | (KRList KRTypDefMethT),Some p => Some (makeModule_meths p)
+                            | _,_ => None
+                            end
+  | KRMakeModule_regs e => match typ,@KRRealizeExp (KRList KRTypModuleElt) e with
+                            | (KRList KRTypRegInitT),Some p => Some (makeModule_regs p)
+                            | _,_ => None
+                            end
+  | KRRegisters l => match typ,@KRRealizeExp (KRList KRTypRegInitT) l with
+                     | KRList KRTypModuleElt,Some p => Some (Registers p)
+                     | _,_ => None
+                     end
+  end.
+  + assert ({t=typ}+{t<>typ}).
+    decide equality.
+    destruct H.
+    - subst.
+      apply (Some e).
+    - apply None.
+  + assert ({t=t0}+{t<>t0}).
+    decide equality.
+    destruct H.
+    - subst.
+      apply (Some (@cons (KRrealizeType t0) f r)).
+    - apply None.
+  + assert ({t=t0}+{t<>t0}).
+    decide equality.
+    destruct H.
+    - subst.
+      apply (Some (@app (KRrealizeType t0) f r)).
+    - apply None.
+Defined.
+
+Definition KRDenote {typ} e def :=
+  match @KRRealizeExp typ e with
+  | Some x => x
+  | _ => def
   end.
 
 Ltac KRReifyExp e t :=
   match e with
   | nil => constr:(@KRNil t)
-  | cons ?F ?R => match t with
-                  | KRList ?T => constr:(@KRCons T (ltac:(KRReifyExp F T)) (ltac:(KRReifyExp R t)))
+  | cons ?F nil => match t with
+                  | KRList ?T => let fr :=ltac:(KRReifyExp F T) in
+                                 constr:(@KRCons T fr (@KRNil T))
                   | ?T => constr:(@KRVar t e)
                   end
-  | app ?F ?R => match t with
-                 | KRList ?T => constr:(@KRApp T (ltac:(KRReifyExp F t)) (ltac:(KRReifyExp R t)))
+  | cons ?F ?R => match t with
+                  | KRList ?T => let fr :=ltac:(KRReifyExp F T) in
+                                 let re:=ltac:(KRReifyExp R t) in
+                                 constr:(@KRCons T fr re)
+                  | ?T => constr:(@KRVar t e)
+                  end
+  | app ?F ?R => let x1 := ltac:(KRReifyExp F t) in
+                 let x2 := ltac:(KRReifyExp R t) in
+                 match t with
+                 | KRList ?T => constr:(@KRApp T x1 x2)
                  | ?T => constr:(@KRVar t e)
                  end
-  | MERegister ?E => match t with
-                     | KRTypModuleElt => constr:(@KRMERegister (ltac:(KRReifyExp E KRTypRegInitT)))
-                     | ?T => constr:(@KRVar t e)
-                     end
-  | Registers ?E => match t with
-                    | KRList KRTypModuleElt => constr:(@KRRegisters (ltac:(KRReifyExp E (KRList KRTypRegInitT))))
-                    | ?T => constr:(@KRVar t e)
-                    end
-  | MERule ?E => match t with
-                 | KRTypModuleElt => constr:(@KRMERule (ltac:(KRReifyExp E KRTypAttributeActionVoid)))
-                 | ?T => constr:(@KRVar t e)
-                 end
-  | MEMeth ?E => match t with
-                 | KRTypModuleElt => constr:(@KRMEMeth (ltac:(KRReifyExp E KRTypDefMethT)))
-                 | ?T => constr:(@KRVar t e)
-                 end
-  | makeModule_rules ?E => match t with
-                           | KRList KRTypAttributeActionVoid => constr:(@KRMakeModule_rules (ltac:(KRReifyExp E (KRList KRTypModuleElt))))
-                           | ?T => constr:(@KRVar t e)
-                           end
-  | makeModule_regs ?E => match t with
-                          | KRList KRTypRegInitT => constr:(@KRMakeModule_regs (ltac:(KRReifyExp E (KRList KRTypModuleElt))))
-                          | ?T => constr:(@KRVar t e)
-                          end
-  | makeModule_meths ?E => match t with
-                          | KRList KRTypDefMethT => constr:(@KRMakeModule_meths (ltac:(KRReifyExp E (KRList KRTypModuleElt))))
-                          | ?T => constr:(@KRVar t e)
-                          end
+  | MERegister ?E => let x := ltac:(KRReifyExp E KRTypRegInitT) in
+                         constr:(@KRMERegister x)
+  | Registers ?E => let x := ltac:(KRReifyExp E (KRList KRTypRegInitT)) in
+                       constr:(@KRRegisters x)
+  | MERule ?E => let  x := ltac:(KRReifyExp E KRTypAttributeActionVoid) in
+                     constr:(@KRMERule x)
+  | MEMeth ?E => let x := ltac:(KRReifyExp E KRTypDefMethT) in
+                     constr:(@KRMEMeth x)
+  | makeModule_rules ?E => let x := ltac:(KRReifyExp E (KRList KRTypModuleElt)) in
+                               constr:(@KRMakeModule_rules x)
+  | makeModule_regs ?X => let x := ltac:(KRReifyExp X (KRList KRTypModuleElt)) in
+                              constr:(@KRMakeModule_regs x)
+  | makeModule_meths ?E => let x := ltac:(KRReifyExp E (KRList KRTypModuleElt)) in 
+                              constr:(@KRMakeModule_meths x)
   | ?X => constr:(@KRVar t X)
   end.
 
-Fixpoint KRSimplifyTop {t} (e : KRExp t) :=
-  match e in KRExp t return KRExp t with
-  | @KRApp KRTypModuleElt f c => match f with
-                                 | @KRCons KRTypModuleElt a b => @KRCons KRTypModuleElt a (@KRApp KRTypModuleElt b c)
-                                 | _ => @KRApp KRTypModuleElt f c
-                                 end
-  | KRRegisters x => match x with
-                     | @KRApp KRTypRegInitT a b => @KRApp KRTypModuleElt (KRRegisters a) (KRRegisters b)
-                     | @KRCons KRTypRegInitT a b => @KRCons KRTypModuleElt (KRMERegister a) (KRRegisters b)
-                     | KRNil KRTypModuleElt => KRNil KRTypModuleElt
-                     | e => KRRegisters e
-                     end
-  | e => e
+
+
+Axiom cheat: forall x, x.
+
+(*Fixpoint KRSimplifyTop2 t' (x:KRExp t'): KRExp t'.
+  refine
+  match x in KRExp t' return KRExp t' with
+  | KRNil t => KRNil t
+  | KRVar t e => KRVar t e
+  | KRCons t a b => KRCons a b
+  | KRApp t a b => match a in KRExp (KRList t') return
+                         KRExp (KRList t') -> KRExp (KRList t') with
+                   | KRCons t'' a' b' => fun b => KRCons a' (KRApp b' b)
+                   | KRNil t => fun b => b
+                   | KRVar _ _ => cheat _
+                   | q => fun b => KRApp q b
+                   end b
+  (* | KRVar t e => e *)
+  (* | KRCons t a b => @cons (@KRrealizeType t) (@KRRealizeExp t a) (@KRRealizeExp (KRList t) b) *)
+  (* | KRApp t a b => @app (@KRrealizeType t) (@KRRealizeExp (KRList t) a) (@KRRealizeExp (KRList t) b) *)
+  (* | KRMERegister e => MERegister (@KRRealizeExp KRTypRegInitT e) *)
+  (* | KRMERule r => MERule (@KRRealizeExp KRTypAttributeActionVoid r) *)
+  (* | KRMEMeth m => MEMeth (@KRRealizeExp KRTypDefMethT m) *)
+  (* | KRMakeModule_rules r => makeModule_rules (KRRealizeExp r) *)
+  (* | KRMakeModule_regs r => makeModule_regs (KRRealizeExp r) *)
+  (* | KRMakeModule_meths m =>makeModule_meths (KRRealizeExp m) *)
+                     (* | KRRegisters l => Registers (KRRealizeExp l) *)
+  | _ => cheat _
   end.
 
-Fixpoint KRSimplify {t} (e: KRExp t) :=
-  match e in KRExp t return KRExp t with
+  (*| @KRApp tp a b => match tp in KRTyp return KRTyp with
+                     | KRTypModuleElt => @KRApp KRTypRegInitT (KRMakeModule_regs a) (KRMakeModule_regs b)
+                     | _ => @KRMakeModule_regs x
+                     end*)
+  (*| @KRCons KRTypRegInitT aa  b => match aa in (KRExp KRTypRegInitT) with
+                                   | KRMERegister a => @KRCons KRTypRegInitT a (KRMakeModule_regs b)
+                                   | _ => @KRMakeModule_regs x
+                                   end*)
+  | @KRNil tp => cheat _
+      (*match tp return KRExp (KRList KRTypRegInitT) with
+                 | _ => @KRMa
+                 end*)
+  | _ => @KRMakeModule_regs x
+  end.
+                 (*| KRTypModuleElt => @KRNil KRTypRegInitT*)
+  *)
+
+Fixpoint KRSimplifyTop (e : KRExp) :=
+  match e with
+  | KRApp tp (KRCons tp2 a b) c => KRCons tp a (KRApp tp b c)
+  | KRRegisters (KRApp KRTypRegInitT a b) => KRApp KRTypModuleElt (KRRegisters a) (KRRegisters b)
+  | KRRegisters (KRCons KRTypRegInitT a b) => KRCons KRTypModuleElt (KRMERegister a) (KRRegisters b)
+  | KRRegisters (KRNil KRTypRegInitT) => KRNil KRTypModuleElt
+  | KRMakeModule_regs (KRNil KRTypModuleElt) => KRNil KRTypRegInitT
+  | KRMakeModule_regs (KRCons KRTypModuleElt (KRMERegister a) b) => KRCons KRTypRegInitT a (KRMakeModule_regs b)
+  | KRMakeModule_regs (KRApp KRTypModuleElt a b) => KRApp KRTypRegInitT (KRMakeModule_regs a) (KRMakeModule_regs b)
+  | _ => e
+  end.
+
+Fixpoint KRSimplify (e: KRExp) :=
+  match e with
   | @KRCons t a b => KRSimplifyTop (@KRCons t (KRSimplify a) (KRSimplify b))
   | @KRApp t a b => KRSimplifyTop (@KRApp t (KRSimplify a) (KRSimplify b))
   | @KRMERegister a => KRSimplifyTop (@KRMERegister (KRSimplify a))
@@ -122,23 +238,51 @@ Fixpoint KRSimplify {t} (e: KRExp t) :=
   end.
 
 
-Theorem KRSimplifySound: forall t e, @KRRealizeExp t e = @KRRealizeExp t (@KRSimplify t e).
+Theorem KRSimplifySound: forall t e d, @KRDenote t e d = @KRDenote t (@KRSimplify e) d.
 Admitted.
 
 Ltac KRSimplifyTac t e :=
   match goal with
   | |- ?A = ?B =>
       let x := (ltac:(KRReifyExp e t)) in
-          replace A with (KRRealizeExp x);[(rewrite KRSimplifySound;compute) | (compute;reflexivity)]
+          replace A with (KRRealizeExp x);[(rewrite KRSimplifySound;cbv [KRRealizeExp]) | (cbv [KRSimplify KRSimplifyTop];reflexivity)]
   end.
   (*let x := ltac:(KRReifyExp e) in
-      (replace e with (KRRealizeExp x);[compute;reflexivity | replace (KRRealizeExp x) with (KRRealizeExp (KRSimplify x));[rewrite KRSimplifySound;reflexivity | compute]]).
+      (replace e with (KRRealizeExp x);[cbv [KRSimplify KRSimplifySound];reflexivity | replace (KRRealizeExp x) with (KRRealizeExp (KRSimplify x));[rewrite KRSimplifySound;reflexivity | compute]]).
 *)
 
-Goal forall a b c d e, makeModule_regs [MERegister a;MERule b;MEMeth c;MERegister d]=e.
+Check KRDenote.
+
+Goal forall a b c d e, Registers ([a;b]++[c;d])=e.
   intros.
-  KRSimplifyTac (KRList KRTypRegInitT) (makeModule_regs [MERegister a;MERule b;MEMeth c;MERegister d]).
+  (*match goal with
+  | |- ?A = ?B => 
+      let x := (ltac:(KRReifyExp A (KRList KRTypRegInitT))) in
+          replace A with (KRRealizeExp x);[(rewrite KRSimplifySound;cbv [KRRealizeExp KRSimplify KRSimplifyTop]) | cbv [KRRealizeExp];reflexivity]
+  end.*)
+  match goal with
+  | |- ?A = ?B => 
+      let x := (ltac:(KRReifyExp A (KRList KRTypModuleElt))) in
+          change A with (@KRDenote (KRList KRTypModuleElt) x nil);rewrite KRSimplifySound
+  end.
+  cbv [KRSimplify KRSimplifyTop KRDenote KRRealizeExp].
 Abort.
+
+(*Goal forall a b c d e, makeModule_regs [MERegister a;MERule b;MEMeth c;MERegister d]=e.
+  intros.
+  (*match goal with
+  | |- ?A = ?B => 
+      let x := (ltac:(KRReifyExp A (KRList KRTypRegInitT))) in
+          replace A with (KRRealizeExp x);[(rewrite KRSimplifySound;cbv [KRRealizeExp KRSimplify KRSimplifyTop]) | cbv [KRRealizeExp];reflexivity]
+  end.*)
+  match goal with
+  | |- ?A = ?B => 
+      let x := (ltac:(KRReifyExp A (KRList KRTypRegInitT))) in
+          change A with (KRRealizeExp x);rewrite KRSimplifySound
+  end.
+  cbv [KRSimplify KRSimplifyTop KRRealizeExp].
+
+Abort.*)
 
 (*Fixpoint KRSimplifyTop {t} (e : KRExp t) :=
   match e in KRExp t return KRExp t with
